6.27

AReg.thy
@@ -11,12 +11,8 @@ inductive_set star :: "'v list set \<Rightarrow> 'v list set"
 zero[intro!]:"[] \<in> star r"|
 step[intro!]:"x \<in> r \<and> y \<in> star r \<Longrightarrow> x@y \<in> star r"
 
-thm star.simps
-
-
-
 primrec sem_reg :: "('v) regexp => 'v set\<Rightarrow> 'v list set" where 
-"sem_reg ESet v = {}"| (*Empty Set*)
+"sem_reg ESet v = {[]}"| (*Empty Set*)
 "sem_reg (Dot) vset = (\<lambda>x .[x]) ` vset" | 
 "sem_reg (Concat r1 r2) v ={q@p| q p. q \<in> sem_reg r1 v \<and> p \<in> sem_reg r2 v}"|
 "sem_reg (LChr a) v = {[a]}"|
